finith network

src/AFP/Network.thy
@@ -42,15 +42,17 @@ lemma (in node_histories) node_total_order_trans:
   assumes "e1 \<sqsubset>\<^sup>i e2"
       and "e2 \<sqsubset>\<^sup>i e3"
     shows "e1 \<sqsubset>\<^sup>i e3"
-  using assms unfolding history_order_def
-  apply clarsimp
-  apply(rename_tac xs1 xs2 ys1 ys2 zs1 zs2)
-  apply(rule_tac x=xs1 in exI, rule_tac x="ys1 @ e2 # ys2" in exI, rule_tac x=zs2 in exI)
-  apply(subgoal_tac "xs1 @ e1 # ys1 = xs2 \<and> zs1 = ys2 @ e3 # zs2")
-   apply clarsimp
-  apply(rule_tac xs="history i" and ys="[e2]" in pre_suf_eq_distinct_list)
-     apply auto
-  done
+proof - 
+  obtain xs1 xs2 ys1 ys2 zs1 zs2 where *: "xs1 @ e1 # ys1 @ e2 # zs1 = history i" "xs2 @ e2 # ys2 @ e3 # zs2 = history i"
+    using history_order_def assms by auto
+  hence "xs1 @ e1 # ys1 = xs2 \<and> zs1 = ys2 @ e3 # zs2"
+    by(rule_tac xs="history i" and ys="[e2]" in pre_suf_eq_distinct_list) auto
+  thus ?thesis
+    apply(clarsimp simp: history_order_def)
+    apply(rule_tac x=xs1 in exI, rule_tac x="ys1 @ e2 # ys2" in exI, rule_tac x=zs2 in exI)
+    using * apply clarsimp
+    done
+qed
 
 lemma (in node_histories) local_order_carrier_closed:
   assumes "e1 \<sqsubset>\<^sup>i e2"
@@ -122,40 +124,39 @@ lemma (in node_histories) local_order_prefix_closed:
       and "xs prefix of i"
       and "y \<in> set xs"
     shows "x \<in> set xs"
-  using assms
-  apply -
-  apply (frule prefix_distinct)
-  apply (insert histories_distinct[where i=i])
-  apply (clarsimp simp: history_order_def prefix_of_node_history_def)
-  apply(rename_tac xs1 ys ys1 zs)
-  apply (frule split_list)
-  apply clarsimp
-  apply(rename_tac ys2 zs2)
-  apply (subgoal_tac "ys2 = xs1 @ x # ys1 \<and> zs2 @ ys = zs")
-   apply clarsimp
-  apply (rule_tac xs="history i" and ys="[y]" in pre_suf_eq_distinct_list)
-     apply auto
-  done
+proof -
+  obtain ys where "xs @ ys = history i"
+    using assms prefix_of_node_history_def by blast
+  moreover obtain as bs cs where "as @ x # bs @ y # cs = history i"
+    using assms history_order_def by blast
+  moreover obtain pre suf where *: "xs = pre @ y # suf"
+    using assms split_list by fastforce
+  ultimately have "pre = as @ x # bs \<and> suf @ ys = cs"
+    by (rule_tac xs="history i" and ys="[y]" in pre_suf_eq_distinct_list) auto
+  thus ?thesis
+    using assms * by clarsimp
+qed
 
 lemma (in node_histories) local_order_prefix_closed_last:
   assumes "x \<sqsubset>\<^sup>i y"
       and "xs@[y] prefix of i"
     shows "x \<in> set xs"
-  using assms
-  apply -
-  apply(frule local_order_prefix_closed, assumption, force)
-  apply(auto simp add: node_total_order_irrefl prefix_to_carriers)
-  done
+proof -
+  have "x \<in> set (xs @ [y])"
+    using assms by (force dest: local_order_prefix_closed)
+  thus ?thesis
+    using assms by(force simp add: node_total_order_irrefl prefix_to_carriers)
+qed
 
 lemma (in node_histories) events_before_exist:
   assumes "x \<in> set (history i)"
   shows "\<exists>pre. pre @ [x] prefix of i"
-  using assms unfolding prefix_of_node_history_def
-  apply -
-  apply(subgoal_tac "\<exists>idx. idx < length (history i) \<and> (history i) ! idx = x")
-   apply(metis append_take_drop_id  take_Suc_conv_app_nth)
-  apply(simp add: set_elem_nth)
-  done
+proof -
+  have "\<exists>idx. idx < length (history i) \<and> (history i) ! idx = x"
+    using assms by(simp add: set_elem_nth)
+  thus ?thesis
+    by(metis append_take_drop_id take_Suc_conv_app_nth prefix_of_node_history_def)
+qed
 
 lemma (in node_histories) events_in_local_order:
   assumes "pre @ [e2] prefix of i"
@@ -217,9 +218,9 @@ text\<open>Based on the well-known definition by \cite{Lamport:1978jq}, we say t
     \end{enumerate}\<close>
 
 inductive (in network) hb :: "'msg \<Rightarrow> 'msg \<Rightarrow> bool" where
-  "\<lbrakk> Broadcast m1 \<sqsubset>\<^sup>i Broadcast m2 \<rbrakk> \<Longrightarrow> hb m1 m2" |
-  "\<lbrakk> Deliver m1 \<sqsubset>\<^sup>i Broadcast m2 \<rbrakk> \<Longrightarrow> hb m1 m2" |
-  "\<lbrakk> hb m1 m2; hb m2 m3 \<rbrakk> \<Longrightarrow> hb m1 m3"
+  hb_broadcast: "\<lbrakk> Broadcast m1 \<sqsubset>\<^sup>i Broadcast m2 \<rbrakk> \<Longrightarrow> hb m1 m2" |
+  hb_deliver:   "\<lbrakk> Deliver m1 \<sqsubset>\<^sup>i Broadcast m2 \<rbrakk> \<Longrightarrow> hb m1 m2" |
+  hb_trans:     "\<lbrakk> hb m1 m2; hb m2 m3 \<rbrakk> \<Longrightarrow> hb m1 m3"
   
 inductive_cases (in network) hb_elim: "hb x y"
         
@@ -261,16 +262,10 @@ lemma (in causal_network) hb_has_a_reason:
   assumes "hb m1 m2"
     and "Broadcast m2 \<in> set (history i)"
   shows "Deliver m1 \<in> set (history i) \<or> Broadcast m1 \<in> set (history i)"
-  using assms
-  apply(induction rule: hb.induct)
+  using assms apply (induction rule: hb.induct)
     apply(metis insert_subset local_order_carrier_closed network.broadcasts_unique network_axioms)
    apply(metis insert_subset local_order_carrier_closed network.broadcasts_unique network_axioms)
-  apply(case_tac "Deliver m2 \<in> set (history i)")
-   apply(subgoal_tac "Deliver m1 \<in> set (history i)")
-    apply blast
-  using causal_delivery local_order_carrier_closed apply blast
-  apply(subgoal_tac "Broadcast m2 \<in> set (history i)")
-   apply blast+
+  using hb_trans causal_delivery local_order_carrier_closed apply blast
   done
 
 lemma (in causal_network) hb_cross_node_delivery:
@@ -283,50 +278,55 @@ lemma (in causal_network) hb_cross_node_delivery:
   apply(induction rule: hb.induct)
     apply(metis broadcasts_unique insert_subset local_order_carrier_closed)
    apply(metis insert_subset local_order_carrier_closed network.broadcasts_unique network_axioms)
-  apply(case_tac "Deliver m2 \<in> set (history j)")
-   apply(subgoal_tac "Deliver m1 \<in> set (history j)")
-    apply blast
   using broadcasts_unique hb.intros(3) hb_has_a_reason apply blast
-  apply(subgoal_tac "Broadcast m2 \<in> set (history j)")
-   apply blast
-  using hb_has_a_reason apply blast      
   done
     
 lemma (in causal_network) hb_irrefl:
   assumes "hb m1 m2"
   shows "m1 \<noteq> m2"
-  using assms
-  apply(induction rule: hb.induct)
-  using node_total_order_antisym apply blast
-   apply(meson causal_broadcast insert_subset local_order_carrier_closed node_total_order_irrefl)
-  apply(subgoal_tac "\<exists>i. Broadcast m3 \<in> set (history i)")
-   apply(subgoal_tac "\<exists>j. Broadcast m2 \<in> set (history j)")
-    apply clarsimp
-    apply(subgoal_tac "Deliver m2 \<in> set (history j) \<and> Deliver m3 \<in> set (history i)")
-     apply(meson causal_delivery hb.intros(3) insert_subset local_order_carrier_closed
-            network.broadcast_before_delivery network_axioms node_total_order_irrefl)
-    apply(meson deliver_locally insert_subset local_order_carrier_closed)
-   apply(simp add: hb_broadcast_exists2)+
-  done
+using assms proof(induction rule: hb.induct)
+  case (hb_broadcast m1 i m2) thus ?case
+    using node_total_order_antisym by blast
+next
+  case (hb_deliver m1 i m2) thus ?case
+    by(meson causal_broadcast insert_subset local_order_carrier_closed node_total_order_irrefl)
+next
+  case (hb_trans m1 m2 m3)
+  then obtain i j where "Broadcast m3 \<in> set (history i)" "Broadcast m2 \<in> set (history j)"
+    using hb_broadcast_exists2 by blast
+  then show ?case
+    using assms hb_trans by (meson causal_network.causal_delivery causal_network_axioms
+        deliver_locally insert_subset network.hb.intros(3) network_axioms 
+        node_histories.local_order_carrier_closed assms hb_trans
+        node_histories_axioms node_total_order_irrefl)
+qed
 
 lemma (in causal_network) hb_broadcast_broadcast_order:
   assumes "hb m1 m2"
     and "Broadcast m1 \<in> set (history i)"
     and "Broadcast m2 \<in> set (history i)"
   shows "Broadcast m1 \<sqsubset>\<^sup>i Broadcast m2"
-  using assms
-  apply(induction rule: hb.induct)
-    apply(metis insertI1 local_order_carrier_closed network.broadcasts_unique network_axioms subsetCE)
-   apply(metis broadcasts_unique insert_subset local_order_carrier_closed
+using assms proof(induction rule: hb.induct)
+  case (hb_broadcast m1 i m2) thus ?case
+    by(metis insertI1 local_order_carrier_closed network.broadcasts_unique network_axioms subsetCE)
+next
+  case (hb_deliver m1 i m2) thus ?case
+    by(metis broadcasts_unique insert_subset local_order_carrier_closed
           network.broadcast_before_delivery network_axioms node_total_order_trans)
-  apply(case_tac "Broadcast m2 \<in> set (history i)")
-  using node_total_order_trans apply blast
-  apply(subgoal_tac "Deliver m2 \<in> set (history i)")
-   apply(subgoal_tac "m1 \<noteq> m2 \<and> m2 \<noteq> m3")
-    apply(metis event.inject(1) hb.intros(1) hb_irrefl network.hb.intros(3) network_axioms node_order_is_total hb_irrefl)
-  using hb_has_a_reason apply blast+
-  done
-
+next
+  case (hb_trans m1 m2 m3)
+  then show ?case
+  proof (cases "Broadcast m2 \<in> set (history i)")
+    case True thus ?thesis
+      using hb_trans node_total_order_trans by blast
+  next
+    case False hence "Deliver m2 \<in> set (history i)" "m1 \<noteq> m2" "m2 \<noteq> m3"
+      using hb_has_a_reason hb_trans by auto
+    thus ?thesis
+      by(metis hb_trans event.inject(1) hb.intros(1) hb_irrefl network.hb.intros(3) network_axioms node_order_is_total hb_irrefl)
+  qed
+qed
+  
 lemma (in causal_network) hb_antisym:
   assumes "hb x y"
       and "hb y x"
@@ -375,6 +375,10 @@ lemma (in network) node_deliver_messages_empty [simp]:
   shows "node_deliver_messages [] = []"
   by(auto simp add: node_deliver_messages_def List.map_filter_simps)
 
+lemma (in network) node_deliver_messages_Cons:
+  shows "node_deliver_messages (x#xs) = (node_deliver_messages [x])@(node_deliver_messages xs)"
+  by(auto simp add: node_deliver_messages_def map_filter_def)
+    
 lemma (in network) node_deliver_messages_append:
   shows "node_deliver_messages (xs@ys) = (node_deliver_messages xs)@(node_deliver_messages ys)"
   by(auto simp add: node_deliver_messages_def map_filter_def)
@@ -391,10 +395,7 @@ lemma (in network) prefix_msg_in_history:
   assumes "es prefix of i"
       and "m \<in> set (node_deliver_messages es)"
     shows "Deliver m \<in> set (history i)"
-  using assms
-  apply(clarsimp simp: node_deliver_messages_def map_filter_def split: event.split_asm)
-  using prefix_to_carriers apply auto
-  done
+using assms prefix_to_carriers by(fastforce simp: node_deliver_messages_def map_filter_def split: event.split_asm)
 
 lemma (in network) prefix_contains_msg:
   assumes "es prefix of i"
@@ -405,55 +406,42 @@ lemma (in network) prefix_contains_msg:
 lemma (in network) node_deliver_messages_distinct:
   assumes "xs prefix of i"
   shows "distinct (node_deliver_messages xs)"
-  using assms
-  apply(induction xs rule: rev_induct, simp)
-  apply(clarsimp simp add: node_deliver_messages_append)
-  apply safe
-    apply force
-   apply(clarsimp simp: node_deliver_messages_def map_filter_def)
-  apply(frule prefix_distinct)
-  apply(clarsimp simp add: map_filter_def node_deliver_messages_def)
-  apply(rename_tac a xs b c)
-  apply(case_tac a; clarsimp)
-  apply(case_tac b; clarsimp)
-  done
-
+using assms proof(induction xs rule: rev_induct)
+  case Nil thus ?case by simp
+next
+  case (snoc x xs)
+  { fix y assume *: "y \<in> set (node_deliver_messages xs)" "y \<in> set (node_deliver_messages [x])"
+    moreover have "distinct (xs @ [x])"
+      using assms snoc prefix_distinct by blast
+    ultimately have "False"
+      using assms apply(case_tac x; clarsimp simp add: map_filter_def node_deliver_messages_def)
+      using * prefix_contains_msg snoc.prems by blast
+  } thus ?case
+    using snoc by(fastforce simp add: node_deliver_messages_append node_deliver_messages_def map_filter_def)
+qed
+  
 lemma (in network) drop_last_message:
   assumes "evts prefix of i"
   and "node_deliver_messages evts = msgs @ [last_msg]"
   shows "\<exists>pre. pre prefix of i \<and> node_deliver_messages pre = msgs"
-  using assms
-  apply -
-  apply(subgoal_tac "\<exists>pre suf. evts = pre @ (Deliver last_msg) # suf \<and> node_deliver_messages suf = []")
-   apply(erule exE)+
-   apply(simp)
-   apply(rule_tac x=pre in exI)
-   apply(rule conjI)
-  using prefix_of_appendD apply blast
-   apply(subgoal_tac "node_deliver_messages ([Deliver last_msg] @ suf) = [last_msg]")
-    apply(simp add: node_deliver_messages_append)
-   apply(metis append_Nil2 node_deliver_messages_append node_deliver_messages_Deliver)
-  apply(subgoal_tac "Deliver last_msg \<in> set evts")
-   apply(subgoal_tac "\<exists>idx. idx < length evts \<and> evts ! idx = Deliver last_msg")
-    apply(erule exE)
-    apply(subgoal_tac "\<exists>pre suf. evts = pre @ (evts ! idx) # suf")
-  defer
-  using list_nth_split_technical id_take_nth_drop apply blast
-    apply(simp add: set_elem_nth)
-      apply(simp add: prefix_contains_msg)
-  apply(erule exE)+
-  apply(rule_tac x=pre in exI, rule_tac x=suf in exI)
-  apply(rule conjI, simp, simp)
-  apply(subgoal_tac "node_deliver_messages (pre @ Deliver last_msg # suf) =
-         (node_deliver_messages pre) @ (node_deliver_messages (Deliver last_msg # suf))")
-  apply(subgoal_tac "node_deliver_messages ([Deliver last_msg] @ suf) = [last_msg] @ []")
-  apply(metis node_deliver_messages_Deliver node_deliver_messages_append self_append_conv)
-  apply(auto simp add: node_deliver_messages_append)
-  apply(subgoal_tac "node_deliver_messages ([Deliver last_msg] @ suf) = [last_msg] @ []")
-  apply(simp add: node_deliver_messages_append)
-  apply(metis append_Cons node_deliver_messages_Deliver node_deliver_messages_append
-    node_deliver_messages_distinct not_Cons_self2 pre_suf_eq_distinct_list self_append_conv2)
-done
+proof -
+  have "Deliver last_msg \<in> set evts"
+    using assms network.prefix_contains_msg network_axioms by force
+  then obtain idx where *: "idx < length evts" "evts ! idx = Deliver last_msg"
+    by (meson set_elem_nth)
+  then obtain pre suf where "evts = pre @ (evts ! idx) # suf"
+    using id_take_nth_drop by blast
+  hence **: "evts = pre @ (Deliver last_msg) # suf"
+    using assms * by auto
+  moreover hence "distinct (node_deliver_messages ([Deliver last_msg] @ suf))"
+    by (metis assms(1) assms(2) distinct_singleton node_deliver_messages_Cons node_deliver_messages_Deliver
+        node_deliver_messages_append node_deliver_messages_distinct not_Cons_self2 pre_suf_eq_distinct_list)
+  ultimately have "node_deliver_messages ([Deliver last_msg] @ suf) = [last_msg] @ []"
+    by (metis append_self_conv assms(1) assms(2) node_deliver_messages_Cons node_deliver_messages_Deliver
+        node_deliver_messages_append node_deliver_messages_distinct not_Cons_self2 pre_suf_eq_distinct_list)
+  thus ?thesis
+    using assms * ** by (metis append1_eq_conv append_Cons append_Nil node_deliver_messages_append prefix_of_appendD)
+qed
 
 locale network_with_ops = causal_network history fst
   for history :: "nat \<Rightarrow> ('msgid \<times> 'op) event list" +
@@ -504,59 +492,55 @@ lemma (in network_with_ops) apply_operations_Deliver [simp]:
 lemma (in network_with_ops) hb_consistent_technical:
   assumes "\<And>m n. m < length cs \<Longrightarrow> n < m \<Longrightarrow> cs ! n \<sqsubset>\<^sup>i cs ! m"
   shows   "hb.hb_consistent (node_deliver_messages cs)"
-  using assms
-  apply -
-  apply(induction cs rule: rev_induct)
-   apply(unfold node_deliver_messages_def)
-   apply(simp add: hb.hb_consistent.intros(1) map_filter_simps(2))
-  apply(case_tac x; clarify)
-   apply(simp add: List.map_filter_def)
-   apply(subgoal_tac "(\<And>m n. m < length xs \<Longrightarrow> n < m \<Longrightarrow> xs ! n \<sqsubset>\<^sup>i xs ! m)")
-    apply clarsimp
-   apply(erule_tac x=m in meta_allE, erule_tac x=n in meta_allE, clarsimp simp add: nth_append)
-  apply(subst map_filter_append)
-  apply(clarsimp simp add: map_filter_def)
-  apply(rule hb.hb_consistent.intros)
-  apply(subgoal_tac "(\<And>m n. m < length xs \<Longrightarrow> n < m \<Longrightarrow> xs ! n \<sqsubset>\<^sup>i xs ! m)")
-  apply clarsimp
-  apply(erule_tac x=m in meta_allE, erule_tac x=n in meta_allE, clarsimp simp add: nth_append)
-  apply clarsimp
-  apply(case_tac x; clarsimp)
-  apply(drule set_elem_nth, erule exE, erule conjE)
-  apply(erule_tac x="length xs" in meta_allE, erule_tac x=m in meta_allE)
-  apply clarsimp
-  apply(subst (asm) nth_append, simp)
-  apply(meson causal_network.causal_delivery causal_network_axioms insert_subset node_histories.local_order_carrier_closed node_histories_axioms node_total_order_irrefl node_total_order_trans)
-  done
+using assms proof (induction cs rule: rev_induct)
+  case Nil thus ?case
+   by(simp add: node_deliver_messages_def hb.hb_consistent.intros(1) map_filter_simps(2))
+next
+  case (snoc x xs)
+  hence *: "(\<And>m n. m < length xs \<Longrightarrow> n < m \<Longrightarrow> xs ! n \<sqsubset>\<^sup>i xs ! m)"
+    by(-, erule_tac x=m in meta_allE, erule_tac x=n in meta_allE, clarsimp simp add: nth_append)
+  then show ?case
+  proof (cases x)
+    case (Broadcast x1) thus ?thesis
+      using snoc * by (simp add: node_deliver_messages_append)
+  next
+    case (Deliver x2) thus ?thesis
+      using snoc * apply(clarsimp simp add: node_deliver_messages_def map_filter_def map_filter_append)
+      apply (rename_tac m m1 m2)
+      apply (case_tac m; clarsimp)
+      apply(drule set_elem_nth, erule exE, erule conjE)
+      apply(erule_tac x="length xs" in meta_allE)
+      apply(clarsimp simp add: nth_append)
+      by (metis causal_delivery insert_subset node_histories.local_order_carrier_closed
+          node_histories_axioms node_total_order_antisym)
+  qed
+qed
     
 corollary (in network_with_ops)
   shows "hb.hb_consistent (node_deliver_messages (history i))"
-  apply(subgoal_tac "history i = [] \<or> (\<exists>c. history i = [c]) \<or> (length (history i) \<ge> 2)")
-   apply(erule disjE, clarsimp simp add: node_deliver_messages_def map_filter_def)+
-    apply blast
-   apply(cases "history i"; clarsimp)
-   apply (rename_tac x xs)
-   apply (case_tac xs; clarsimp)
-   apply(rule hb_consistent_technical[where i=i])                                         
-  apply(subst history_order_def, clarsimp)
-  apply(metis list_nth_split One_nat_def Suc_le_mono cancel_comm_monoid_add_class.diff_cancel
-          le_imp_less_Suc length_Cons less_Suc_eq_le less_imp_diff_less neq0_conv nth_Cons_pos)
-  apply (metis Suc_leI Suc_pred length_0_conv length_Suc_conv neq0_conv numeral_2_eq_2 zero_less_diff)
-  done
+  by (metis hb_consistent_technical history_order_def less_one linorder_neqE_nat list_nth_split zero_order(3))
 
 lemma (in network_with_ops) hb_consistent_prefix:
   assumes "xs prefix of i"
   shows "hb.hb_consistent (node_deliver_messages xs)"
-  using assms proof (clarsimp simp: prefix_of_node_history_def)
-  fix ys assume "xs @ ys = history i"
-  moreover hence "xs = [] \<or> (\<exists>c. xs = [c]) \<or> (length (xs) > 1)"
-    by (metis One_nat_def Suc_pred length_Suc_conv length_greater_0_conv zero_less_diff)
-  ultimately show "hb.hb_consistent (node_deliver_messages xs)"
-    apply(rule_tac i=i in hb_consistent_technical)
-    apply(erule disjE, clarsimp)+
-    apply(drule list_nth_split, assumption, clarsimp)
-    apply (metis append.assoc append.simps(2) history_order_def)
-    done
+using assms proof (clarsimp simp: prefix_of_node_history_def, rule_tac i=i in hb_consistent_technical)
+  fix m n ys assume *: "xs @ ys = history i" "m < length xs" "n < m"
+  consider (a) "xs = []" | (b) "\<exists>c. xs = [c]" | (c) "Suc 0 < length (xs)"
+    by (metis Suc_pred length_Suc_conv length_greater_0_conv zero_less_diff)
+  thus "xs ! n \<sqsubset>\<^sup>i xs ! m"
+  proof (cases)
+    case a thus ?thesis
+      using * by clarsimp
+  next
+    case b thus ?thesis
+      using assms * by clarsimp
+  next
+    case c thus ?thesis
+      using assms * apply clarsimp
+      apply(drule list_nth_split, assumption, clarsimp simp: c)
+      apply (metis append.assoc append.simps(2) history_order_def)
+      done
+  qed
 qed
 
 locale network_with_constrained_ops = network_with_ops +
